<?xml version="1.0" encoding="utf-8"?>
<rdf:RDF
  xmlns:dcterms="http://purl.org/dc/terms/"
  xmlns:foaf="http://xmlns.com/foaf/0.1/"
  xmlns:owl="http://www.w3.org/2002/07/owl#"
  xmlns:prv="http://purl.org/net/provenance/ns#"
  xmlns:rdf="http://www.w3.org/1999/02/22-rdf-syntax-ns#"
  xmlns:rdfs="http://www.w3.org/2000/01/rdf-schema#"
  xmlns:wot="http://xmlns.com/wot/0.1/"
  xmlns:xhv="http://www.w3.org/1999/xhtml/vocab#"
  xmlns:xml="http://www.w3.org/XML/1998/namespace"
  xmlns:xsd="http://www.w3.org/2001/XMLSchema#"
>
  <owl:ObjectProperty rdf:about="http://purl.org/net/provenance/ns#containedBy">
    <rdfs:label xml:lang="en">contained in</rdfs:label>
    <rdfs:comment xml:lang="en">This property refers to a data item that contained a data item. Hence, this property refers to another data item of a larger granularity (e.g. an RDF statement is usually contained in an RDF graph).</rdfs:comment>
    <rdfs:isDefinedBy>
      <owl:Ontology rdf:about="http://purl.org/net/provenance/ns#">
        <dcterms:description xml:lang="en">The Provenance Vocabulary provides classes and properties to describe the provenance of data from the Web. Hence, this vocabulary enables providers of Web data to publish provenance-related metadata about their data. The Provenance Vocabulary Core Ontology provides the main classes and properties required to describe provenance of data on the Web. Notice, this vocabulary is not designed to describe provenance of other kinds of content such as documents.</dcterms:description>
        <dcterms:creator>
          <foaf:Person rdf:about="http://olafhartig.de/foaf.rdf#olaf">
            <foaf:name xml:lang="en">Olaf Hartig</foaf:name>
            <foaf:homepage>
              <foaf:Document rdf:about="http://olafhartig.de/"/>
            </foaf:homepage>
          </foaf:Person>
        </dcterms:creator>
        <dcterms:creator>
          <foaf:Person rdf:about="http://users.ox.ac.uk/~zool0770/foaf.rdf#me">
            <foaf:name xml:lang="en">Jun Zhao</foaf:name>
            <foaf:homepage>
              <foaf:Document rdf:about="http://users.ox.ac.uk/~zool0770/"/>
            </foaf:homepage>
          </foaf:Person>
        </dcterms:creator>
        <dcterms:created rdf:datatype="http://www.w3.org/2001/XMLSchema#dateTime">2010-07-10T12:00:00Z</dcterms:created>
        <dcterms:title xml:lang="en">Provenance Vocabulary Core Ontology namespace</dcterms:title>
      </owl:Ontology>
    </rdfs:isDefinedBy>
    <rdfs:range>
      <owl:Class rdf:about="http://purl.org/net/provenance/ns#DataItem">
        <owl:disjointWith>
          <owl:Class rdf:about="http://purl.org/net/provenance/ns#File">
            <owl:disjointWith rdf:resource="http://purl.org/net/provenance/ns#DataItem"/>
            <rdfs:label xml:lang="en">File</rdfs:label>
            <rdfs:comment xml:lang="en">File is a general class that represents computer files/documents of any kind.</rdfs:comment>
            <rdfs:subClassOf>
              <owl:Class rdf:about="http://purl.org/net/provenance/ns#Artifact">
                <owl:disjointWith>
                  <owl:Class rdf:about="http://purl.org/net/provenance/ns#Actor">
                    <rdfs:comment xml:lang="en">Actor is a general class that represents active entities. Actors usually perform the execution (see the class Execution) of an action or a process.</rdfs:comment>
                    <rdfs:label xml:lang="en">Actor</rdfs:label>
                    <owl:equivalentClass rdf:resource="http://xmlns.com/foaf/0.1/Agent"/>
                    <rdfs:isDefinedBy rdf:resource="http://purl.org/net/provenance/ns#"/>
                  </owl:Class>
                </owl:disjointWith>
                <owl:disjointWith>
                  <owl:Class rdf:about="http://purl.org/net/provenance/ns#Execution">
                    <owl:disjointWith rdf:resource="http://purl.org/net/provenance/ns#Artifact"/>
                    <owl:disjointWith rdf:resource="http://purl.org/net/provenance/ns#Actor"/>
                    <rdfs:label xml:lang="en">Execution</rdfs:label>
                    <rdfs:comment xml:lang="en">Execution is a general class that represents completed executions of actions or processes. An execution is usually performed by an actor (see the class Actor) and an execution, in most cases, yielded an artifact (see the class Artifact).</rdfs:comment>
                    <rdfs:subClassOf rdf:nodeID="ZStZwuRO7"/>
                    <rdfs:isDefinedBy rdf:resource="http://purl.org/net/provenance/ns#"/>
                  </owl:Class>
                </owl:disjointWith>
                <rdfs:label xml:lang="en">Artifact</rdfs:label>
                <rdfs:comment xml:lang="en">Artifact is a general class that represents artifacts which can be used during the execution (see the class Execution) of an action or a process and which can also be the result of such an execution.</rdfs:comment>
                <rdfs:subClassOf>
                  <owl:Restriction>
                    <owl:maxCardinality rdf:datatype="http://www.w3.org/2001/XMLSchema#nonNegativeInteger">1</owl:maxCardinality>
                    <owl:onProperty rdf:resource="http://purl.org/net/provenance/ns#retrievedBy"/>
                  </owl:Restriction>
                </rdfs:subClassOf>
                <rdfs:isDefinedBy rdf:resource="http://purl.org/net/provenance/ns#"/>
              </owl:Class>
            </rdfs:subClassOf>
            <rdfs:isDefinedBy rdf:resource="http://purl.org/net/provenance/ns#"/>
          </owl:Class>
        </owl:disjointWith>
        <rdfs:label xml:lang="en">Data Item</rdfs:label>
        <rdfs:comment xml:lang="en">DataItem is a general class that represents any kind of representation of a data item.</rdfs:comment>
        <rdfs:subClassOf rdf:resource="http://purl.org/net/provenance/ns#Artifact"/>
        <rdfs:subClassOf>
          <owl:Class rdf:about="http://www.ontologydesignpatterns.org/cp/owl/informationrealization.owl#InformationRealization"/>
        </rdfs:subClassOf>
        <rdfs:isDefinedBy rdf:resource="http://purl.org/net/provenance/ns#"/>
      </owl:Class>
    </rdfs:range>
    <rdfs:domain rdf:resource="http://purl.org/net/provenance/ns#DataItem"/>
  </owl:ObjectProperty>
  <owl:ObjectProperty rdf:about="http://purl.org/dc/terms/creator"/>
  <foaf:Document rdf:about="http://purl.org/net/provenance/ns.rdf"/>
  <owl:ObjectProperty rdf:about="http://xmlns.com/wot/0.1/assurance"/>
  <owl:ObjectProperty rdf:about="http://xmlns.com/wot/0.1/endorser"/>
  <owl:Class rdf:about="http://www.ontologydesignpatterns.org/ont/web/irw.owl#WebServer">
    <rdfs:subClassOf>
      <owl:Class rdf:about="http://purl.org/net/provenance/ns#DataProvidingService">
        <rdfs:comment xml:lang="en">DataProvidingService is a class that represents a non-human actor - usually a Web service or a server (software) - that processes data access requests and actually sends the requested Web representations over the Web.</rdfs:comment>
        <rdfs:label xml:lang="en">Data Providing Service</rdfs:label>
        <rdfs:isDefinedBy rdf:resource="http://purl.org/net/provenance/ns#"/>
        <rdfs:subClassOf>
          <owl:Class rdf:about="http://purl.org/net/provenance/ns#NonHumanActor">
            <owl:disjointWith>
              <owl:Class rdf:about="http://purl.org/net/provenance/ns#HumanActor">
                <owl:disjointWith rdf:resource="http://purl.org/net/provenance/ns#Artifact"/>
                <owl:disjointWith rdf:resource="http://purl.org/net/provenance/ns#Execution"/>
                <owl:disjointWith rdf:resource="http://purl.org/net/provenance/ns#NonHumanActor"/>
                <rdfs:label xml:lang="en">Human Actor</rdfs:label>
                <rdfs:comment xml:lang="en">HumanActor is a general class that represents actors who are social beings such as persons, organizations, companies.</rdfs:comment>
                <rdfs:subClassOf rdf:resource="http://purl.org/net/provenance/ns#Actor"/>
                <rdfs:isDefinedBy rdf:resource="http://purl.org/net/provenance/ns#"/>
              </owl:Class>
            </owl:disjointWith>
            <rdfs:label xml:lang="en">Non-Human Actor</rdfs:label>
            <rdfs:comment xml:lang="en">NonHumanActor is a general class that represents actors who are not social beings.</rdfs:comment>
            <rdfs:subClassOf rdf:resource="http://purl.org/net/provenance/ns#Actor"/>
            <rdfs:isDefinedBy rdf:resource="http://purl.org/net/provenance/ns#"/>
          </owl:Class>
        </rdfs:subClassOf>
      </owl:Class>
    </rdfs:subClassOf>
  </owl:Class>
  <owl:ObjectProperty rdf:about="http://purl.org/dc/terms/conformsTo"/>
  <owl:Class rdf:about="http://xmlns.com/foaf/0.1/Group">
    <rdfs:subClassOf rdf:resource="http://purl.org/net/provenance/ns#HumanActor"/>
  </owl:Class>
  <foaf:Document rdf:about="http://trdf.sourceforge.net/provenance/ns.html">
    <dcterms:conformsTo>
      <owl:Thing rdf:about="http://www.w3.org/TR/rdfa-syntax"/>
    </dcterms:conformsTo>
    <wot:assurance>
      <wot:Endorsement rdf:about="http://trdf.sourceforge.net/provenance/ns.html.sig">
        <wot:endorser>
          <wot:PubKey rdf:about="http://olafhartig.de/foaf.rdf#pubkey2009"/>
        </wot:endorser>
        <dcterms:title xml:lang="en">Detached signature</dcterms:title>
      </wot:Endorsement>
    </wot:assurance>
    <rdfs:label xml:lang="en">Document that defines the core ontology of the Provenance Vocabulary</rdfs:label>
    <xhv:alternate rdf:resource="http://trdf.sourceforge.net/provenance/ns.rdf"/>
    <dcterms:description xml:lang="en">This documents specifies the classes and properties introduced by the Provenance Vocabulary Core Ontology.</dcterms:description>
    <foaf:primaryTopic rdf:resource="http://purl.org/net/provenance/ns#"/>
    <xhv:license>
      <owl:Thing rdf:about="http://creativecommons.org/licenses/by/1.0/"/>
    </xhv:license>
    <dcterms:title xml:lang="en">Provenance Vocabulary Core Ontology Specification</dcterms:title>
  </foaf:Document>
  <owl:DeprecatedProperty rdf:about="http://purl.org/net/provenance/ns#encodedBy">
    <rdf:type rdf:resource="http://www.w3.org/2002/07/owl#ObjectProperty"/>
    <rdfs:label xml:lang="en">encoded by</rdfs:label>
    <rdfs:comment xml:lang="en">This property is deprecated and will be removed from the Provenance Vocabulary shortly. Use prv:serializedBy instead. prv:encodedBy was deprecated because the new name prv:serializedBy is more suitable.</rdfs:comment>
    <rdfs:isDefinedBy rdf:resource="http://purl.org/net/provenance/ns#"/>
    <rdfs:range rdf:resource="http://purl.org/net/provenance/ns#File"/>
    <rdfs:domain rdf:resource="http://purl.org/net/provenance/ns#DataItem"/>
  </owl:DeprecatedProperty>
  <owl:DatatypeProperty rdf:about="http://purl.org/dc/terms/description"/>
  <owl:ObjectProperty rdf:about="http://www.w3.org/1999/xhtml/vocab#license"/>
  <owl:DeprecatedClass rdf:about="http://purl.org/net/provenance/ns#Representation">
    <rdf:type rdf:resource="http://www.w3.org/2002/07/owl#Class"/>
    <owl:disjointWith rdf:resource="http://purl.org/net/provenance/ns#DataItem"/>
    <owl:disjointWith rdf:resource="http://purl.org/net/provenance/ns#File"/>
    <rdfs:label xml:lang="en">Web Representation</rdfs:label>
    <rdfs:comment xml:lang="en">This class is deprecated and will be removed from the Provenance Vocabulary in the next revision. Use prv:DataItem instead. prv:Representation was deprecated because the Provenance Vocabulary does not distinguish Web representations of data and the general kind of representations (as prv:DataItem represents).</rdfs:comment>
    <rdfs:subClassOf rdf:resource="http://purl.org/net/provenance/ns#Artifact"/>
    <rdfs:subClassOf>
      <owl:Class rdf:about="http://www.ontologydesignpatterns.org/ont/web/irw.owl#WebRepresentation"/>
    </rdfs:subClassOf>
    <rdfs:subClassOf>
      <owl:Class rdf:about="http://sw.nokia.com/WebArch-1/Representation"/>
    </rdfs:subClassOf>
    <owl:equivalentClass rdf:resource="http://purl.org/net/provenance/ns#DataItem"/>
    <rdfs:isDefinedBy rdf:resource="http://purl.org/net/provenance/ns#"/>
  </owl:DeprecatedClass>
  <owl:ObjectProperty rdf:about="http://purl.org/net/provenance/ns#performedBy">
    <rdfs:subPropertyOf>
      <owl:ObjectProperty rdf:about="http://purl.org/net/provenance/ns#involvedActor">
        <rdfs:label xml:lang="en">involved</rdfs:label>
        <rdfs:comment xml:lang="en">This is an abstract property that refers to an actor involved in an execution.</rdfs:comment>
        <rdfs:isDefinedBy rdf:resource="http://purl.org/net/provenance/ns#"/>
        <rdfs:range rdf:resource="http://purl.org/net/provenance/ns#Actor"/>
        <rdfs:domain rdf:resource="http://purl.org/net/provenance/ns#Execution"/>
      </owl:ObjectProperty>
    </rdfs:subPropertyOf>
    <rdfs:label xml:lang="en">performed by</rdfs:label>
    <rdfs:comment xml:lang="en">This property refers to an actor that/who performed an execution.</rdfs:comment>
    <rdfs:isDefinedBy rdf:resource="http://purl.org/net/provenance/ns#"/>
    <rdfs:range rdf:resource="http://purl.org/net/provenance/ns#Actor"/>
    <rdfs:domain rdf:resource="http://purl.org/net/provenance/ns#Execution"/>
  </owl:ObjectProperty>
  <owl:DatatypeProperty rdf:about="http://purl.org/dc/terms/created"/>
  <owl:ObjectProperty rdf:about="http://purl.org/net/provenance/ns#usedGuideline">
    <rdfs:subPropertyOf>
      <owl:ObjectProperty rdf:about="http://purl.org/net/provenance/ns#usedData">
        <rdfs:subPropertyOf>
          <owl:ObjectProperty rdf:about="http://purl.org/net/provenance/ns#employedArtifact">
            <rdfs:label xml:lang="en">used</rdfs:label>
            <rdfs:comment xml:lang="en">This is an abstract property that refers to an artifact which was used during an execution.</rdfs:comment>
            <rdfs:isDefinedBy rdf:resource="http://purl.org/net/provenance/ns#"/>
            <rdfs:range rdf:resource="http://purl.org/net/provenance/ns#Artifact"/>
            <rdfs:domain rdf:resource="http://purl.org/net/provenance/ns#Execution"/>
          </owl:ObjectProperty>
        </rdfs:subPropertyOf>
        <rdfs:label xml:lang="en">used</rdfs:label>
        <rdfs:comment xml:lang="en">This property refers to a source data item that has been used during the creation of a data item. Examples for source data are the content of a document used for machine learning, the statements in a knowledge base used to entail a new statement, and the entries in a database used to answer a query. Notice, all source data has provenance; we strongly encourage to describe this provenance as well, at least as far as available information permits.</rdfs:comment>
        <rdfs:isDefinedBy rdf:resource="http://purl.org/net/provenance/ns#"/>
        <rdfs:seeAlso rdf:resource="http://purl.org/net/provenance/files#"/>
        <rdfs:range rdf:resource="http://purl.org/net/provenance/ns#DataItem"/>
        <rdfs:domain>
          <owl:Class rdf:about="http://purl.org/net/provenance/ns#DataCreation">
            <owl:disjointWith>
              <owl:Class rdf:about="http://purl.org/net/provenance/ns#DataAccess">
                <owl:disjointWith rdf:resource="http://purl.org/net/provenance/ns#DataCreation"/>
                <rdfs:label xml:lang="en">Data Access</rdfs:label>
                <rdfs:comment xml:lang="en">DataAccess is a class that represents the completed execution of accessing a data item on the Web.</rdfs:comment>
                <rdfs:subClassOf>
                  <owl:Restriction>
                    <owl:maxCardinality rdf:datatype="http://www.w3.org/2001/XMLSchema#nonNegativeInteger">1</owl:maxCardinality>
                    <owl:onProperty rdf:resource="http://purl.org/net/provenance/ns#accessedService"/>
                  </owl:Restriction>
                </rdfs:subClassOf>
                <rdfs:subClassOf rdf:resource="http://purl.org/net/provenance/ns#Execution"/>
                <rdfs:subClassOf>
                  <owl:Restriction>
                    <owl:maxCardinality rdf:datatype="http://www.w3.org/2001/XMLSchema#nonNegativeInteger">1</owl:maxCardinality>
                    <owl:onProperty rdf:resource="http://purl.org/net/provenance/ns#accessedResource"/>
                  </owl:Restriction>
                </rdfs:subClassOf>
                <rdfs:isDefinedBy rdf:resource="http://purl.org/net/provenance/ns#"/>
              </owl:Class>
            </owl:disjointWith>
            <rdfs:label xml:lang="en">Data Creation</rdfs:label>
            <rdfs:comment xml:lang="en">DataCreation is a class that represents the completed creation of a data item.</rdfs:comment>
            <rdfs:subClassOf rdf:resource="http://purl.org/net/provenance/ns#Execution"/>
            <rdfs:isDefinedBy rdf:resource="http://purl.org/net/provenance/ns#"/>
          </owl:Class>
        </rdfs:domain>
      </owl:ObjectProperty>
    </rdfs:subPropertyOf>
    <rdfs:label xml:lang="en">guided by</rdfs:label>
    <rdfs:comment xml:lang="en">This property refers to a creation guideline which guided the execution of a data creation. Examples for creation guidelines are transformation rules, mapping definitions, entailment rules, and database queries. Notice, all creation guidelines have provenance; we strongly encourage to describe this provenance as well, at least as far as available information permits.</rdfs:comment>
    <rdfs:isDefinedBy rdf:resource="http://purl.org/net/provenance/ns#"/>
    <rdfs:seeAlso rdf:resource="http://purl.org/net/provenance/files#"/>
    <rdfs:range>
      <owl:Class rdf:about="http://purl.org/net/provenance/ns#CreationGuideline">
        <rdfs:comment xml:lang="en">CreationGuideline is a class that represents a guideline used to guide the execution of a data creation. Examples for creation guidelines are transformation rules, mapping definitions, entailment rules, and database queries.</rdfs:comment>
        <rdfs:label xml:lang="en">Creation Guideline</rdfs:label>
        <rdfs:isDefinedBy rdf:resource="http://purl.org/net/provenance/ns#"/>
        <rdfs:subClassOf rdf:resource="http://purl.org/net/provenance/ns#DataItem"/>
      </owl:Class>
    </rdfs:range>
    <rdfs:domain rdf:resource="http://purl.org/net/provenance/ns#DataCreation"/>
  </owl:ObjectProperty>
  <owl:ObjectProperty rdf:about="http://purl.org/net/provenance/ns#precededBy">
    <rdfs:subPropertyOf>
      <owl:ObjectProperty rdf:about="http://purl.org/dc/terms/replaces"/>
    </rdfs:subPropertyOf>
    <rdfs:label xml:lang="en">immediately preceded by</rdfs:label>
    <rdfs:comment xml:lang="en">This property refers to an immediately preceding version of a data item; hence, the new version (i.e. the subject) has been created using the old version (i.e. the object). We strongly encourage to also describe this creation of the new version explicitly.</rdfs:comment>
    <rdfs:isDefinedBy rdf:resource="http://purl.org/net/provenance/ns#"/>
    <rdfs:range rdf:resource="http://purl.org/net/provenance/ns#DataItem"/>
    <rdfs:domain rdf:resource="http://purl.org/net/provenance/ns#DataItem"/>
  </owl:ObjectProperty>
  <owl:ObjectProperty rdf:about="http://www.w3.org/1999/xhtml/vocab#alternate"/>
  <owl:ObjectProperty rdf:about="http://purl.org/net/provenance/ns#deployedSoftware">
    <rdfs:comment xml:lang="en">This property refers to the software that was run by a non-human actor (usually a service).</rdfs:comment>
    <rdfs:label xml:lang="en">runs</rdfs:label>
    <rdfs:isDefinedBy rdf:resource="http://purl.org/net/provenance/ns#"/>
    <rdfs:domain rdf:resource="http://purl.org/net/provenance/ns#NonHumanActor"/>
  </owl:ObjectProperty>
  <owl:Class rdf:about="http://xmlns.com/foaf/0.1/Organization">
    <rdfs:subClassOf rdf:resource="http://purl.org/net/provenance/ns#HumanActor"/>
  </owl:Class>
  <owl:ObjectProperty rdf:about="http://xmlns.com/foaf/0.1/primaryTopic"/>
  <owl:ObjectProperty rdf:about="http://purl.org/net/provenance/ns#usedBy">
    <rdfs:label xml:lang="en">used by</rdfs:label>
    <rdfs:comment xml:lang="en">This property refers to a data publisher who used a data providing services at the time the provenance description refers to.</rdfs:comment>
    <rdfs:isDefinedBy rdf:resource="http://purl.org/net/provenance/ns#"/>
    <rdfs:range>
      <owl:Class rdf:about="http://purl.org/net/provenance/ns#DataPublisher">
        <rdfs:comment xml:lang="en">DataPublisher is a class that represents entities such as persons, groups, or organizations who use a data providing service (see class prv:DataProvidingService) to publish data on the Web.</rdfs:comment>
        <rdfs:label xml:lang="en">Data Publisher</rdfs:label>
        <rdfs:isDefinedBy rdf:resource="http://purl.org/net/provenance/ns#"/>
        <rdfs:subClassOf rdf:resource="http://purl.org/net/provenance/ns#HumanActor"/>
      </owl:Class>
    </rdfs:range>
    <rdfs:domain rdf:resource="http://purl.org/net/provenance/ns#DataProvidingService"/>
  </owl:ObjectProperty>
  <owl:Class rdf:about="http://sw.nokia.com/WebArch-1/Server">
    <rdfs:subClassOf rdf:resource="http://purl.org/net/provenance/ns#DataProvidingService"/>
  </owl:Class>
  <owl:ObjectProperty rdf:about="http://xmlns.com/foaf/0.1/homepage"/>
  <owl:DatatypeProperty rdf:about="http://purl.org/dc/terms/title"/>
  <owl:DatatypeProperty rdf:about="http://xmlns.com/foaf/0.1/name"/>
  <owl:ObjectProperty rdf:about="http://purl.org/net/provenance/ns#operatedBy">
    <rdfs:label xml:lang="en">operated by</rdfs:label>
    <rdfs:comment xml:lang="en">This property refers to a human actor who was operating a non-human actor at the time the provenance description refers to. For instance, a service provider operated a data providing service (see class prv:DataProvidingService). Another example is a human actor who operated a non-human data creating actor.</rdfs:comment>
    <rdfs:isDefinedBy rdf:resource="http://purl.org/net/provenance/ns#"/>
    <rdfs:range rdf:resource="http://purl.org/net/provenance/ns#HumanActor"/>
    <rdfs:domain rdf:resource="http://purl.org/net/provenance/ns#NonHumanActor"/>
  </owl:ObjectProperty>
  <owl:Class rdf:about="http://sw.nokia.com/WebArch-1/Service">
    <rdfs:subClassOf rdf:resource="http://purl.org/net/provenance/ns#DataProvidingService"/>
  </owl:Class>
  <owl:Class rdf:about="http://xmlns.com/wot/0.1/Endorsement"/>
  <owl:Class rdf:nodeID="ZStZwuRO11">
    <owl:unionOf rdf:parseType="Collection">
      <rdf:Description rdf:about="http://purl.org/net/provenance/ns#DataItem"/>
      <rdf:Description rdf:about="http://purl.org/net/provenance/ns#File"/>
    </owl:unionOf>
  </owl:Class>
  <owl:Class rdf:about="http://xmlns.com/foaf/0.1/Document"/>
  <owl:ObjectProperty rdf:about="http://purl.org/net/provenance/ns#serializedBy">
    <rdfs:comment xml:lang="en">This property refers to a file that serialized a data item.</rdfs:comment>
    <rdfs:label xml:lang="en">serialized by</rdfs:label>
    <rdfs:range rdf:resource="http://purl.org/net/provenance/ns#File"/>
    <rdfs:isDefinedBy rdf:resource="http://purl.org/net/provenance/ns#"/>
  </owl:ObjectProperty>
  <owl:DatatypeProperty rdf:about="http://purl.org/net/provenance/ns#performedAt">
    <rdfs:label xml:lang="en">executed at</rdfs:label>
    <rdfs:comment xml:lang="en">This property refers to the time an execution has been performed at.</rdfs:comment>
    <rdfs:isDefinedBy rdf:resource="http://purl.org/net/provenance/ns#"/>
    <rdfs:range rdf:resource="http://www.w3.org/2001/XMLSchema#dateTime"/>
    <rdfs:domain rdf:resource="http://purl.org/net/provenance/ns#Execution"/>
  </owl:DatatypeProperty>
  <owl:ObjectProperty rdf:about="http://purl.org/net/provenance/ns#accessedService">
    <rdfs:subPropertyOf rdf:resource="http://purl.org/net/provenance/ns#involvedActor"/>
    <rdfs:label xml:lang="en">accessed</rdfs:label>
    <rdfs:comment xml:lang="en">This property refers to the service that provided the Web representation during the execution of a data access.</rdfs:comment>
    <rdfs:isDefinedBy rdf:resource="http://purl.org/net/provenance/ns#"/>
    <rdfs:range rdf:resource="http://purl.org/net/provenance/ns#DataProvidingService"/>
    <rdfs:domain rdf:resource="http://purl.org/net/provenance/ns#DataAccess"/>
  </owl:ObjectProperty>
  <owl:ObjectProperty rdf:about="http://purl.org/net/provenance/ns#retrievedBy">
    <rdfs:subPropertyOf>
      <owl:ObjectProperty rdf:about="http://purl.org/net/provenance/ns#yieldedBy">
        <rdfs:label xml:lang="en">yielded by</rdfs:label>
        <rdfs:comment xml:lang="en">This is an abstract property that refers to the execution by which an artifact was yielded.</rdfs:comment>
        <rdfs:isDefinedBy rdf:resource="http://purl.org/net/provenance/ns#"/>
        <rdfs:range rdf:resource="http://purl.org/net/provenance/ns#Execution"/>
        <rdfs:domain rdf:resource="http://purl.org/net/provenance/ns#Artifact"/>
      </owl:ObjectProperty>
    </rdfs:subPropertyOf>
    <rdfs:label xml:lang="en">retrieved by</rdfs:label>
    <rdfs:comment xml:lang="en">This property refers to the data access by which a Web representation of data has been retrieved from the Web.</rdfs:comment>
    <rdfs:isDefinedBy rdf:resource="http://purl.org/net/provenance/ns#"/>
    <rdfs:range rdf:resource="http://purl.org/net/provenance/ns#DataAccess"/>
    <rdfs:domain rdf:resource="http://purl.org/net/provenance/ns#Artifact"/>
  </owl:ObjectProperty>
  <owl:Restriction rdf:nodeID="ZStZwuRO7">
    <owl:maxCardinality rdf:datatype="http://www.w3.org/2001/XMLSchema#nonNegativeInteger">1</owl:maxCardinality>
    <owl:onProperty rdf:resource="http://purl.org/net/provenance/ns#performedAt"/>
  </owl:Restriction>
  <owl:Class rdf:about="http://xmlns.com/wot/0.1/PubKey"/>
  <owl:ObjectProperty rdf:about="http://purl.org/net/provenance/ns#accessedResource">
    <rdfs:subPropertyOf rdf:resource="http://purl.org/net/provenance/ns#employedArtifact"/>
    <rdfs:label xml:lang="en">accessed</rdfs:label>
    <rdfs:comment xml:lang="en">This property refers to the Web resource that has been accessed during the execution of a data access. More precisely, the request of the referenced Web resource resulted in retrieving the representation that has been retrieved by the corresponding prv:DataAccess execution.</rdfs:comment>
    <rdfs:isDefinedBy rdf:resource="http://purl.org/net/provenance/ns#"/>
    <rdfs:range>
      <owl:Class rdf:about="http://www.ontologydesignpatterns.org/ont/web/irw.owl#WebResource"/>
    </rdfs:range>
    <rdfs:domain rdf:resource="http://purl.org/net/provenance/ns#DataAccess"/>
  </owl:ObjectProperty>
  <owl:Class rdf:about="http://xmlns.com/foaf/0.1/Agent"/>
  <rdfs:List rdf:nodeID="ZStZwuRO17">
    <rdf:first rdf:resource="http://purl.org/net/provenance/ns#serializedBy"/>
    <rdf:rest/>
  </rdfs:List>
  <owl:ObjectProperty rdf:about="http://purl.org/net/provenance/ns#createdBy">
    <rdfs:subPropertyOf rdf:resource="http://purl.org/net/provenance/ns#yieldedBy"/>
    <rdfs:label xml:lang="en">created by</rdfs:label>
    <rdfs:comment xml:lang="en">This property refers to the creation of a data item.</rdfs:comment>
    <owl:propertyChainAxiom rdf:parseType="Collection">
      <rdf:Description rdf:about="http://purl.org/net/provenance/ns#serializedBy"/>
      <rdf:Description rdf:about="http://purl.org/net/provenance/ns#createdBy"/>
    </owl:propertyChainAxiom>
    <rdfs:isDefinedBy rdf:resource="http://purl.org/net/provenance/ns#"/>
    <rdfs:range rdf:resource="http://purl.org/net/provenance/ns#DataCreation"/>
    <rdfs:domain rdf:nodeID="ZStZwuRO11"/>
  </owl:ObjectProperty>
  <owl:Class rdf:about="http://xmlns.com/foaf/0.1/Person">
    <rdfs:subClassOf rdf:resource="http://purl.org/net/provenance/ns#HumanActor"/>
  </owl:Class>
</rdf:RDF>
